Fad/Chapter3.lean
@@ -1,0 +1,65 @@
+
+namespace Chapter3
+
+open List (reverse tail cons)
+
+-- 3.1 Symmetric lists
+
+def snoc {a : Type u} (x : a) (xs : List a) : List a :=
+  xs ++ [x]
+
+def SymList (α : Type u) := (List α) × (List α)
+
+def nilSL : SymList a := ([], [])
+
+def fromSL (sl : SymList a) : List a :=
+ sl.1 ++ sl.2.reverse
+
+def snocSL : a → SymList a → SymList a
+| z, ([],    ys) => (ys, [z])
+| z, (b::bs, ys) => (b::bs, z :: ys)
+
+def consSL : a → SymList a → SymList a
+| z, (xs, []) => ([z], xs)
+| z, (xs, ys) => (z :: xs, ys)
+
+#eval fromSL $ consSL 4 $ consSL 3 $ consSL 2 $ consSL 1 nilSL
+
+def lastSL : SymList a → Option a
+| (xs, ys) => if ys.isEmpty then xs.head? else ys.head?
+
+#eval fromSL (snocSL 1 (snocSL 2 (snocSL 3 ([], []))))
+
+def _root_.List.splitAt (xs : List a) (n : Nat) : List a × List a :=
+ (xs.take n, xs.drop n)
+
+#eval [1, 2, 3, 4, 5].splitAt 2
+
+def tailSL (sl : SymList a) : Option (SymList a) :=
+ let (us, vs) := sl.2.splitAt (sl.2.length / 2)
+ match sl with
+ | ([],       []) => none
+ | ([],  _ :: []) => some nilSL
+ | (_ :: [],   _) => some (reverse vs, us)
+ | (xs,       ys) => some (tail xs, ys)
+
+#eval tailSL (snocSL 1 (snocSL 2 (snocSL 3 ([], []))))
+#eval do let a ← tailSL (snocSL 1 (snocSL 2 (snocSL 3 ([], [])))); pure $ fromSL a
+
+#check pure ∘ fromSL
+#eval tailSL (snocSL 1 (snocSL 2 (snocSL 3 ([], [])))) >>= pure ∘ fromSL
+
+-- Evidencias como argumentos
+
+/- https://lean-lang.org/functional_programming_in_lean/props-proofs-indexing.html#evidence-as-arguments -/
+
+#eval [].head (by simp)
+#eval [1,2].head (by simp)
+
+def third (xs : List α) (ok : xs.length > 2) : α := xs[2]
+
+#eval third [1, 2, 3, 4] (by decide)
+
+
+
+end Chapter3
